\begin{frame}
	\begin{textblock*}{70mm}(30mm,30mm)
		\begin{greenbox}{}
			\begin{equation*}
			H=g(t,x(t),u(t))+\lambda(t)f(t,x(t),u(t)),
			\end{equation*}
		\end{greenbox}
	\end{textblock*}
	\only<2>
	{
		\begin{textblock*}{120mm}(5mm,50mm)
			\begin{yellowbox}{}
				$$\left\{ \begin{array}{l}
				\dot{x}(s)=f(s,u(s),x(s))\,\,s\in [t_0,T], \\
				x(t_0)=x_0,\\
				\end{array}
				\right.$$			
				$$J(t_0,x_0;u(\cdot))=\int_{t_0}^{T}g(s,u(s),x(s))ds+h(x(T)).$$
			\end{yellowbox}
		\end{textblock*}
	}
	
\end{frame}
%%%%%%%%%%%%%%%%%%%%%%%%%%%%%%%%%%%%%%%%%%%%%%%%%%%%%%%%%%%%%%%%%%%%%%%%%%%%%%%%
\begin{frame}
	\begin{textblock*}{120mm}(5mm,15mm)
		\begin{graybox}{Pontryaginâ€™s Maximum Principle}
			If $u^*(t)$ and $x^*(t)$ are optimal for the problem $(OC)$, then there exists a piecewise differentiable adjoint variable $\lambda(t)$ s.t.
				\begin{equation*}
					H(t,x^*(t),u(t),\lambda(t))\leq H(t,x^*(t),u^*(t),\lambda(t))
				\end{equation*}
			$\forall$ $u$ at $t$,

				\begin{align*}
					\lambda'(t) &= -\frac{\partial H(t,x^*(t),u^*(t),\lambda(t))}{\partial x},\\
					\lambda(T) &= 0.
				\end{align*}
		\end{graybox}
		
	\end{textblock*}
	
\end{frame}

%%%%%%%%%%%%%%%%%%%%%%%%%%%%%%%%%%%%%%%%%%%%%%%%%%%%%%%%%%%%%%%%%%%%%%%%%%%%%%%%
\begin{frame}
		\begin{textblock*}{80mm}(25mm,20mm)
			\begin{greenbox}{}
				\begin{align*}
					H&=A_1I_v+A_2L_p+A_3I_v+\sum_{i=1}^{3}c_iu_i^2\\
					&+\lambda_1(-\beta_p S_p I_v +(r +u_1)L_p + (r + u_2) I_p)\\
					&+\lambda_2(\beta_p S_p I_v -b L_p -(r + u_1)L_p)\\
					&+\lambda_3(b L_p - (r + u_2) I_p)\\
					&+\lambda_4(-\beta_v S_v I_p - (\gamma+u_3) S_v +(1-\theta)\mu)\\
					&+\lambda_5(\beta_v S_v I_p -(\gamma+u_3) I_v +\theta\mu).
				\end{align*}
			\end{greenbox}
		\end{textblock*}
\end{frame}

%%%%%%%%%%%%%%%%%%%%%%%%%%%%%%%%%%%%%%%%%%%%%%%%%%%%%%%%%%%%%%%%%%%%%%%%%%%%%%%%

\begin{frame}[plain]
	\begin{textblock*}{80mm}(25mm,3mm)
		\begin{greenbox}{}
			\begin{align*}
			\frac{d\lambda_1}{dt} &=\beta_p (\lambda_1-\lambda_2),\\
			\frac{d\lambda_2}{dt} &=-A_2+(r+u_1)(\lambda_2-\lambda_1)+b(\lambda_2-\lambda_3),\\
			\frac{d\lambda_3}{dt} &-A_1+(r+u_2)(\lambda_3-\lambda_1)+\beta_vS_v(\lambda_4-\lambda_5),\\
			\frac{d\lambda_4}{dt} &=\beta_v I_p(\lambda_4-\lambda_5)+(\gamma+u_3)\lambda_4,\\
			\frac{d\lambda_5}{dt} &=-A_3+\beta_p S_p(\lambda_1-\lambda_2)+(\gamma+u_3)\lambda_5,				
			\end{align*}
		\end{greenbox}	
	\end{textblock*}
	
	\begin{textblock*}{90mm}(20mm,57mm)
		\begin{yellowbox}{}
			$$u_1^*=\min\left(\max\left(0,\frac{L_p(\lambda_2-\lambda_1)}{2c_1}\right),u_{1_{max}}\right)$$
			$$u_2^*=\min\left(\max\left(0,\frac{I_p(\lambda_3-\lambda_1)}{2c_2}\right),u_{2_{max}}\right)$$
			$$u_3^*=\min\left(\max\left(0,\frac{S_v\lambda_4+I_v\lambda_5}{2c_3}\right),u_{3_{max}}\right)$$
		\end{yellowbox}
		
	\end{textblock*}
	
\end{frame}
%%%%%%%%%%%%%%%%%%%%%%%%%%%%%%%%%%%%%%%%%%%%%%%%%%%%%%%%%%%%%%%%%%%%%%%%%%%%%%%%